proofs/isabelle/SpecRest/core/Smt.thy
@@ -19,6 +19,8 @@ datatype (plugins only: code size) smt_val =
   | SNone
   | SSome "smt_val"
   | SStr "String.literal"
+  | SSeq "smt_val list"
+  | SMap "(smt_val \<times> smt_val) list"
 
 datatype (plugins only: code size) smt_term =
     BLit bool
@@ -57,6 +59,10 @@ datatype (plugins only: code size) smt_term =
   | TNone
   | TSome "smt_term"
   | TStrLit "String.literal"
+  | TSeqEmpty
+  | TSeqCons "smt_term" "smt_term"
+  | TMapEmpty
+  | TMapCons "smt_term" "smt_term" "smt_term"
 
 record smt_model =
   sm_sort_members :: "(String.literal \<times> String.literal list) list"
@@ -324,6 +330,16 @@ where
 | "smtEval m env TNone     = Some SNone"
 | "smtEval m env (TSome t) = map_option SSome (smtEval m env t)"
 | "smtEval m env (TStrLit v) = Some (SStr v)"
+| "smtEval m env TSeqEmpty = Some (SSeq [])"
+| "smtEval m env (TSeqCons e rest) =
+     (case (smtEval m env e, smtEval m env rest) of
+        (Some v, Some (SSeq vs)) \<Rightarrow> Some (SSeq (v # vs))
+      | _ \<Rightarrow> None)"
+| "smtEval m env TMapEmpty = Some (SMap [])"
+| "smtEval m env (TMapCons k v rest) =
+     (case (smtEval m env k, smtEval m env v, smtEval m env rest) of
+        (Some kv, Some vv, Some (SMap ps)) \<Rightarrow> Some (SMap ((kv, vv) # ps))
+      | _ \<Rightarrow> None)"
 
 | "smtEval_forall_enum m env var sort_name [] body = Some (SBool True)"
 | "smtEval_forall_enum m env var sort_name (mem # rest) body =
